add insert_avl2 to F* spec
handle insertion equality case

Trees.fst
@@ -328,7 +328,7 @@ let rec insert_bst2_aux_size (#a: Type)
 let insert_bst2 (#a: Type)
   (r: bool) (cmp:cmp a) (t: bst a cmp) (new_data: a)
   : t':wds a{
-    let new_t, b = insert_bst2_aux r cmp t new_data in
+    let _, b = insert_bst2_aux r cmp t new_data in
   size_of_tree t' == size_of_tree t + (int_of_bool b)}
   =
   insert_bst2_aux_size r cmp t new_data;
@@ -887,6 +887,47 @@ let rec insert_avl (#a: Type) (cmp:cmp a) (x: avl a cmp) (key: a)
     )
 
 (*
+- r: in case of equality with an already existing element,
+  true = replace, false = do not replace
+- snd (result): whether a new element has been added,
+  that is whether the size has increased
+  => bad idea/bad design?
+*)
+
+let rec insert_avl2_aux (#a: Type)
+  (r:bool) (cmp:cmp a) (t: avl a cmp) (new_data: a)
+  : result:(wds a & bool){
+    let t',b = result in
+    size_of_tree t' = size_of_tree t + (int_of_bool b) /\
+    is_wds t'
+  }
+  =
+  match t with
+  | Leaf -> Node new_data Leaf Leaf 1, true
+  | Node data left right size ->
+    let delta = cmp data new_data in
+    if delta = 0 then begin
+      if r
+      then
+        Node new_data left right size, false
+      else
+        t, false
+    end
+    else if delta > 0 then begin
+      let new_left, b = insert_avl2_aux r cmp left new_data in
+      let new_size = size + (int_of_bool b) in
+      let t, b = Node data new_left right new_size, b in
+      rebalance_avl_wds_size t;
+      rebalance_avl_wds t, b
+    end else begin
+      let new_right, b = insert_avl2_aux r cmp right new_data in
+      let new_size = size + (int_of_bool b) in
+      let t, b = Node data left new_right new_size, b in
+      rebalance_avl_wds_size t;
+      rebalance_avl_wds t, b
+    end
+
+(*
 let rec insert_avl_aux_height (#a: Type)
   (cmp: cmp a) (x: avl a cmp) (key: a)
   : Lemma (
@@ -917,10 +958,18 @@ let insert_avl_aux_height2 (#a: Type)
   | Node data left right size -> ()
 *)
 
-#push-options "--fuel 1 --ifuel 1 --z3rlimit 50"
-let rec insert_avl_proof_aux (#a: Type) (cmp:cmp a) (x: avl a cmp) (key: a)
-  (root:a)
+let rec insert_avl2 (#a: Type)
+  (r:bool) (cmp:cmp a) (t: avl a cmp) (new_data: a)
+  : t':wds a{
+    let _,b = insert_avl2_aux r cmp t new_data in
+    size_of_tree t' = size_of_tree t + (int_of_bool b) /\
+    is_wds t'
+  }
+  = fst (insert_avl2_aux r cmp t new_data)
 
+#push-options "--fuel 1 --ifuel 1 --z3rlimit 50"
+let rec insert_avl_proof_aux (#a: Type)
+  (cmp:cmp a) (x: avl a cmp) (key: a) (root:a)
   : Lemma (requires is_avl cmp x)
     (ensures (
       let res = insert_avl cmp x key in
@@ -952,10 +1001,72 @@ let rec insert_avl_proof_aux (#a: Type) (cmp:cmp a) (x: avl a cmp) (key: a)
     )
 #pop-options
 
-let insert_avl_proof (#a: Type) (cmp:cmp a) (x: avl a cmp) (key: a)
-  : Lemma (requires is_avl cmp x) (ensures is_avl cmp (insert_avl cmp x key))
+#push-options "--fuel 1 --ifuel 1 --z3rlimit 100"
+let rec insert_avl2_proof_aux (#a: Type)
+  (r:bool) (cmp:cmp a) (t: avl a cmp) (new_data: a) (root:a)
+  : Lemma (requires is_avl cmp t)
+    (ensures (
+      let res, _ = insert_avl2_aux r cmp t new_data in
+      is_avl cmp res /\
+      height t <= height res /\
+      height res <= height t + 1 /\
+      (forall_keys t (key_left cmp root) /\
+        key_left cmp root new_data
+        ==> forall_keys res (key_left cmp root)) /\
+      (forall_keys t (key_right cmp root) /\
+        key_right cmp root new_data
+        ==> forall_keys res (key_right cmp root)))
+    )
+  =
+  match t with
+  | Leaf -> ()
+  | Node data left right size ->
+    let delta = cmp data new_data in
+    if delta = 0 then begin
+      if r then begin
+        let t = Node new_data left right size in
+        forall_keys_trans left
+          (key_left cmp data) (key_left cmp new_data);
+        forall_keys_trans right
+          (key_right cmp data) (key_right cmp new_data);
+        assert (is_bst cmp t)
+      end else ()
+    end
+    else if delta > 0 then begin
+      let new_left, b = insert_avl2_aux r cmp left new_data in
+      let new_size = size + (int_of_bool b) in
+      let t, b = Node data new_left right new_size, b in
+      insert_avl2_proof_aux r cmp left new_data data;
+      insert_avl2_proof_aux r cmp left new_data root;
+      rebalance_avl_wds_proof cmp t root
+    end else begin
+      let new_right, b = insert_avl2_aux r cmp right new_data in
+      let new_size = size + (int_of_bool b) in
+      let t, b = Node data left new_right new_size, b in
+      insert_avl2_proof_aux r cmp right new_data data;
+      insert_avl2_proof_aux r cmp right new_data root;
+      rebalance_avl_wds_proof cmp t root
+    end
+#pop-options
+
+let insert_avl_proof (#a: Type)
+  (cmp:cmp a) (t: avl a cmp) (new_data: a)
+  : Lemma
+  (requires is_avl cmp t)
+  (ensures is_avl cmp (insert_avl cmp t new_data))
   = Classical.forall_intro (
       Classical.move_requires (
-        insert_avl_proof_aux cmp x key
+        insert_avl_proof_aux cmp t new_data
+      )
+    )
+
+let insert_avl2_proof (#a: Type)
+  (r:bool) (cmp:cmp a) (t: avl a cmp) (new_data: a)
+  : Lemma
+  (requires is_avl cmp t)
+  (ensures is_avl cmp (insert_avl2 r cmp t new_data))
+  = Classical.forall_intro (
+      Classical.move_requires (
+        insert_avl2_proof_aux r cmp t new_data
       )
     )
